trunk/color/RPO/VRPO_Prover.v
@@ -1,0 +1,144 @@
+(**
+CoLoR, a Coq library on rewriting and termination.
+See the COPYRIGHTS and LICENSE files.
+
+- Adam Koprowski, 2007-05-17
+
+  RPO employed for proving termination of concrete examples.
+*)
+
+Require Import ATrs.
+Require VPrecedence.
+Require VRPO_Status.
+Require VRPO_Results.
+Require VTerm_of_ATerm.
+
+Module Type TRPO.
+
+  Parameter Sig : Signature.
+  Parameter stat : Sig -> VRPO_Status.status_name.
+  Parameter prec : Sig -> nat.
+
+End TRPO.
+
+Module RPO_Prover (R : TRPO).
+
+  Export R.
+
+  Notation term := (@term Sig).
+  Notation rule := (@rule Sig).
+  Notation rules := (@list rule).
+
+  Module VPrecedence <: VPrecedence.VPrecedenceType.
+
+    Definition Sig := VTerm_of_ATerm.VSig_of_ASig Sig.
+
+    Notation term := (term Sig).
+    Notation terms := (list term).
+
+    Definition leF f g := prec f <= prec g.
+
+    Definition ltF := Preorder.ltA Sig leF.
+    Definition eqF := Preorder.eqA Sig leF.
+
+    Lemma ltF_wf : well_founded ltF.
+
+    Proof.
+      unfold ltF, Preorder.ltA, Preorder.eqA, leF. simpl.
+      apply WF_wf. (*apply WF_incl with (fun f g => f > g).*)
+    Admitted.
+
+    Lemma ltF_dec : rel_dec ltF.
+
+    Proof.
+    Admitted.
+
+    Lemma leF_preorder : preorder Sig leF.
+
+    Proof.
+    Admitted.
+
+    Infix "=F=" := eqF (at level 50).
+    Infix "<F" := ltF (at level 50).
+    Infix "<=F" := leF (at level 50).
+
+  End VPrecedence.
+
+  Module VRPO_Wf_Model := VRPO_Status.RPO_Wf_Model VPrecedence.
+  Module VRPO_Wf := VRPO_Results.RPO_Wf_Facts VRPO_Wf_Model.
+  Module VRPO := VRPO_Wf_Model.Base.
+
+  Section TerminationCriterion.
+
+    Variable R : rules.
+
+    Definition arpo := Rof (transp VRPO.lt) (@VTerm_of_ATerm.vterm_of_aterm Sig).
+
+    Lemma arpo_dec : rel_dec arpo.
+
+    Proof.
+      intros p q.
+      destruct (VRPO_Wf.rpo_lt_dec (VTerm_of_ATerm.vterm_of_aterm q)
+        (VTerm_of_ATerm.vterm_of_aterm p)); intuition.
+    Defined.
+
+    Lemma Acc_transp_transp : forall (A : Set) (R : relation A), 
+      forall x, Acc R x -> Acc (transp (transp R)) x.
+
+    Proof.
+    Admitted.
+
+    Lemma arpo_wf : WF arpo.
+
+    Proof.
+      intro x. unfold arpo. set (t := VTerm_of_ATerm.vterm_of_aterm x).
+      apply SN_Rof with t; trivial.
+      apply Acc_SN. apply Acc_transp_transp.
+      apply VRPO_Wf.wf_lt.
+    Qed.
+
+    Lemma arpo_subst_closed : substitution_closed arpo.
+
+    Proof.
+      intro t. 
+    Admitted.
+
+    Lemma arpo_context_closed : context_closed arpo.
+
+    Proof.
+      unfold context_closed. intros. induction c.
+      simpl. assumption.
+      simpl fill. apply monotonic_lt.
+      Lemma monotonic_lt : forall f ss ts,
+
+do 2 rewrite term_int_fun.
+do 2 (rewrite Vmap_cast; rewrite Vmap_app). simpl. apply H. exact IHc.
+      
+      unfold context_closed. intros.
+    Admitted.
+
+    Require Import ACompat.
+
+    Definition part_rpo := rule_partition arpo_dec.
+
+    Lemma arpo_rewrite_ordering : rewrite_ordering arpo.
+
+    Proof.
+      constructor. apply arpo_subst_closed. apply arpo_context_closed.
+    Qed.
+
+    Lemma rpo_termination :
+      let R_gt := partition part_rpo R in
+        snd R_gt = nil ->
+        WF (red R).
+
+    Proof.
+      intros. apply WF_incl with arpo.
+      apply compat_red. apply arpo_rewrite_ordering.
+      apply rule_partition_compat with arpo_dec. assumption.
+      apply arpo_wf.
+    Qed.
+
+  End TerminationCriterion.
+
+End RPO_Prover.
